Included dat3m.h to some tests (+ regenerated their .bpl files). Reverted changes made to VisitorBoogie.getFunctionNameFromCallContext

benchmarks/c/miscellaneous/propagatableSideEffects.c
@@ -1,5 +1,6 @@
 #include <stdlib.h>
 #include <assert.h>
+#include "dat3m.h"
 
 // This test makes sure that we do not accidentally cut off side-effect-full loops
 // whose side-effects were propagated by constant propagation
